Initial commit of rewrite_search rewrite
Engine components and "edit_distance" strategy added

src/tidy/rewrite_search.lean
@@ -1,273 +1,66 @@
--- Copyright (c) 2018 Scott Morrison. All rights reserved.
--- Released under Apache 2.0 license as described in the file LICENSE.
--- Authors: Daniel Barter, Louis Carlin, Scott Morrison, Sam Quinn, Simon Hudon
+import .rewrite_search.engine
+import .rewrite_search.strategy.edit_distance
 
-import data.list
-import data.option
-import .edit_distance
-import .pretty_print
-import .rewrite_all
+open tidy.rewrite_search tidy.rewrite_search.strategy
+open interactive interactive.types expr tactic
 
-namespace tidy.rewrite_search
-
-open edit_distance_progress
-open tactic
-
-meta structure expr_delta :=
-  (current : expr)
-  (proof   : expr)
-  (rewrites : list (ℕ × ℕ))
-
-meta structure node :=
-  (lhs rhs               : expr_delta)
-  (lhs_pp rhs_pp         : string)
-  (lhs_tokens rhs_tokens : list string)
-  (distance              : edit_distance_progress lhs_tokens rhs_tokens)
-
-meta def node.to_string (n : node) := n.lhs_pp ++ " = " ++ n.rhs_pp.
-
--- TODO perhaps also store a hash in node, and compare on that first?
-meta def node.equiv (a b : node) : Prop := a.lhs_pp = b.lhs_pp ∧ a.rhs_pp = b.rhs_pp
-
-meta instance : decidable_rel node.equiv := λ a b,
-begin
-    dunfold node.equiv,
-    dunfold id_rhs,
-    clear decidable_rel,
-    by apply_instance,
-end
-
-meta def node.distance_bound (n : node) :=
-match n.distance with
-| exactly _ _ k    := k
-| at_least _ _ k _ := k
-end
-
-meta def node.mk' (lhs rhs : expr_delta) : tactic node :=
-do
-  lhs_pp ← pretty_print lhs.current,
-  rhs_pp ← pretty_print rhs.current,
-  let lhs_tokens := lhs_pp.split_on ' ',
-  let rhs_tokens := rhs_pp.split_on ' ',
-  let distance := at_least lhs_tokens rhs_tokens 0 (empty_partial_edit_distance_data lhs_tokens rhs_tokens),
-  return ⟨ lhs, rhs, lhs_pp, rhs_pp, lhs_tokens, rhs_tokens, distance ⟩
-
-meta def node.mk'' (lhs rhs : expr) : tactic node :=
-do
-  lhs_proof ← mk_eq_refl lhs,
-  rhs_proof ← mk_eq_refl rhs,
-  node.mk' ⟨ lhs, lhs_proof, [] ⟩ ⟨ rhs, rhs_proof, [] ⟩
-
-
-open list
-
-/- `find_first_node_at_distance nodes k` returns the first node in `nodes` that is at distance exactly `k`, if there is one,
-   along with a list of all the other nodes, possibly with their distance bounds improved. -/
-meta def find_first_node_at_distance : list node → ℕ → (option node) × list node
-| nil k      := (none, nil)
-| (h :: t) k := if h.distance_bound = k then
-                  match h.distance with
-                  | exactly _ _ _ := (some h, t)
-                  | at_least _ _ _ d := 
-                      let ed := update_edit_distance h.distance in
-                      if ed = exactly _ _ k then
-                        (some { h with distance := exactly _ _ k }, t)
-                      else
-                        match find_first_node_at_distance t k with
-                          | (o, l) := (o, { h with distance := ed } :: l)
-                          end                      
-                  end
-                else
-                  match find_first_node_at_distance t k with
-                  | (o, l) := (o, h :: l)
-                  end
-
-meta def select_next_aux : list node → ℕ → option (node × (list node))
-| [] _    := none
-| nodes k := match find_first_node_at_distance nodes k with
-                | (some n, r) := some (n, r)
-                | (none, r)   := select_next_aux r (k+1)
-             end
-
-meta def select_next (nodes: list node) : option (node × (list node)) := select_next_aux nodes 0
-
-meta def new_nodes (rs : list (expr × bool)) (seen_nodes : list node) (n : node) : tactic (list node) := 
-do 
-  lhs_rewrites ← all_rewrites_list rs n.lhs.current,
-  lhs_new_nodes ← lhs_rewrites.mmap $ λ lhs', (do prf ← mk_eq_trans n.lhs.proof lhs'.2.1, node.mk' ⟨ lhs'.1, prf, lhs'.2.2 :: n.lhs.rewrites ⟩ n.rhs),
-  rhs_rewrites ← all_rewrites_list rs n.rhs.current,
-  rhs_new_nodes ← rhs_rewrites.mmap $ λ rhs', (do prf ← mk_eq_trans n.rhs.proof rhs'.2.1, node.mk' n.lhs ⟨ rhs'.1, prf, rhs'.2.2 :: n.rhs.rewrites ⟩),
-  let result := ((lhs_new_nodes ++ rhs_new_nodes).filter $ λ m, ∀ m' ∈ seen_nodes, ¬ (m.equiv m')),
-  return result
-
-structure rewrite_search_config :=
-  (trace         : bool := ff)
-  (trace_result  : bool := ff)
-  (trace_rules   : bool := ff)
-  (trace_summary : bool := tt)
-  (max_steps          : option ℕ := none)
-  (max_extra_distance : option ℕ := some 50)
-
-meta def attempt_refl (lhs rhs : expr) : tactic unit :=
-lock_tactic_state $
-do
-  gs ← get_goals,
-  m ← to_expr ``(%%lhs = %%rhs) >>= mk_meta_var,
-  set_goals [m],
-  refl ← mk_const `eq.refl,
-  result ← try_core (tactic.apply_core refl {new_goals := new_goals.non_dep_only}),
-  set_goals gs,
-  guard result.is_some
-
-meta def rewrite_search_core (rs : list (expr × bool)) (cfg : rewrite_search_config := {}) (initial_distance : ℕ) : list node → list node → tactic (ℕ × ℕ × option node)
-| old_nodes active_nodes := 
-   if cfg.max_steps.is_some ∧ old_nodes.length ≥ cfg.max_steps.get_or_else 0 then
-   do
-     trace "max_steps exceeded during rewrite_search",
-     active_nodes.mmap' $ λ m, trace (m.lhs_pp ++ " = " ++ m.rhs_pp ++ ", distance ≥ " ++ (to_string m.distance_bound)),
-     return (old_nodes.length, active_nodes.length, none)
-   else
-      match select_next active_nodes with
-      | none := return (old_nodes.length, active_nodes.length, none)
-      | some (n, r) := 
-        do
-          if cfg.trace then trace format!"rewrite_search considering node: {n.lhs_pp} = {n.rhs_pp}, distance: {n.distance.to_string}" else skip,
-          match n.distance with
-          | (exactly _ _ 0) := return (old_nodes.length, active_nodes.length, some n)
-          | (exactly _ _ k) := 
-            do
-              (attempt_refl n.lhs.current n.rhs.current >> return (old_nodes.length, active_nodes.length, some n)) <|>
-              do
-                if cfg.max_extra_distance.is_some ∧ k > initial_distance + cfg.max_extra_distance.get_or_else 0 then
-                do
-                  trace "max_extra_distance exceeded during rewrite_search",
-                  return (old_nodes.length, active_nodes.length, none)
-                else
-                do 
-                  nn ← new_nodes rs (old_nodes ++ active_nodes) n,
-                  rewrite_search_core (n :: old_nodes) (r ++ nn)
-          | _ := fail "unreachable code!"
-          end
-      end
-
-meta def rewrite_search (rs : list (expr × bool)) (cfg : rewrite_search_config := {}) (lhs rhs : expr) : tactic (ℕ × expr_delta × expr_delta) :=
-do  first_node ← node.mk'' lhs rhs,
-    result ← rewrite_search_core rs cfg (edit_distance_core first_node.distance) [] [first_node],
-    match result with 
-    | (steps, remaining, (some n)) := return (steps, n.lhs, n.rhs)
-    | (_, 0, none)                 := fail "rewrite_search exhausted the rewrite graph"
-    | (_, _, none)                 := fail "rewrite_search stopped because it exceeded a limit"
-    end
-
-meta def explain_proof (rs : list string) (p : expr_delta × expr_delta) : string :=
-let lhs_steps := p.1.rewrites.reverse.map $ λ q, "perform_nth_rewrite_lhs [" ++ (rs.nth q.1).iget ++ "] " ++ (to_string q.2) in
-let rhs_steps := p.2.rewrites.reverse.map $ λ q, "perform_nth_rewrite_rhs [" ++ (rs.nth q.1).iget ++ "] " ++ (to_string q.2) in
-string.intercalate ",\n" (lhs_steps ++ rhs_steps)
-
-meta def explain_proof_concisely (rs : list string) (p : expr_delta × expr_delta) (needs_refl : bool) : string :=
-"erw [" ++ (string.intercalate ", " ((p.1.rewrites.reverse ++ p.2.rewrites.reverse).map $ λ q, (rs.nth q.1).iget)) ++ "]" ++ (if needs_refl then ", refl" else "")
-
--- fails if we can't just use rewrite
--- otherwise, returns 'tt' if we need a `refl` at the end
-meta def check_if_simple_rewrite_succeeds (rs : list (expr × bool)) (p : expr_delta × expr_delta) : tactic bool :=
-lock_tactic_state $
-focus1 $
-do
+meta def do_rewrite_search (rs : list (expr × bool)) (cfg : config := {}) : tactic string := do
   t ← target,
-  let lhs_rewrites : list (expr × bool) := p.1.rewrites.reverse.map $ λ a, (rs.nth a.1).iget,
-  list.mfoldl (λ e : unit, λ q : expr × bool, rewrite_target q.1 {symm := q.2, md := semireducible}) unit.star lhs_rewrites,
-  let rhs_rewrites : list (expr × bool) := p.2.rewrites.reverse.map $ λ a, (rs.nth a.1).iget,
-  list.mfoldl (λ e : unit, λ q : expr × bool, rewrite_target q.1 {symm := q.2, md := semireducible}) unit.star rhs_rewrites,
-  (reflexivity reducible >> return ff) <|> (reflexivity >> return tt)
-  .
+  match t with
+  | `(%%lhs = %%rhs) := do
+    -- if cfg.trace_rules then
+    --   do rs_strings ← pp_rules rs,
+    --     trace ("rewrite_search using:\n---\n" ++ (string.intercalate "\n" rs_strings) ++ "\n---")
+    -- else skip,
+    -- (steps, r1, r2) ← rewrite_search rs cfg lhs rhs,
+    -- if cfg.trace then trace "rewrite_search found proof:" else skip,
+    -- prf2 ← mk_eq_symm r2.proof,
+    -- prf ← mk_eq_trans r1.proof prf2,
+    -- -- if cfg.trace then trace prf else skip,
+    -- rs_strings ← pp_rules rs,
+    -- explanation ← (do 
+    --   needs_refl ← check_if_simple_rewrite_succeeds rs (r1, r2),
+    --   return (explain_proof_concisely rs_strings (r1, r2) needs_refl)) <|> return (explain_proof rs_strings (r1, r2)),
+    -- if cfg.trace_result then trace explanation          
+    -- else skip,
+    -- if cfg.trace_summary then 
+    --   do name ← decl_name,
+    --     trace format!"during elaboration of {name}, rewrite_search considered {steps} expressions, and found a chain of {r1.rewrites.length + r2.rewrites.length} rewrites"
+    -- else skip,
+    -- exact prf,
+    -- return explanation,
 
-meta def pp_rules (rs : list (expr × bool)) : tactic (list string) := rs.mmap (λ p, (do pp ← pretty_print p.1, return (if p.2 then ("←" ++ pp) else pp)))
-
-meta def rewrite_search_target (rs : list (expr × bool)) (cfg : rewrite_search_config := {}) : tactic string :=
-do t ← target,
-   match t with
-   | `(%%lhs = %%rhs) := do
-                           if cfg.trace_rules then
-                             do rs_strings ← pp_rules rs,
-                                trace ("rewrite_search using:\n---\n" ++ (string.intercalate "\n" rs_strings) ++ "\n---")
-                           else skip,
-                           (steps, r1, r2) ← rewrite_search rs cfg lhs rhs,
-                           if cfg.trace then trace "rewrite_search found proof:" else skip,
-                           prf2 ← mk_eq_symm r2.proof,
-                           prf ← mk_eq_trans r1.proof prf2,
-                           if cfg.trace then trace prf else skip,
-                           rs_strings ← pp_rules rs,
-                           explanation ← (do 
-                             needs_refl ← check_if_simple_rewrite_succeeds rs (r1, r2),
-                              return (explain_proof_concisely rs_strings (r1, r2) needs_refl)) <|> return (explain_proof rs_strings (r1, r2)),
-                           if cfg.trace_result then trace explanation          
-                           else skip,
-                           if cfg.trace_summary then 
-                             do name ← decl_name,
-                                trace format!"during elaboration of {name}, rewrite_search considered {steps} expressions, and found a chain of {r1.rewrites.length + r2.rewrites.length} rewrites"
-                           else skip,
-                           exact prf,
-                           return explanation
-   | _ := fail "target is not an equation"
-   end
-
-end tidy.rewrite_search
+    let strat := edit_distance_strategy,
+    i ← mk_search_instance cfg rs strat lhs rhs,
+    result ← i.search_until_abort,
+    match result with
+      | search_result.success str    := return str
+      | search_result.failure reason := fail reason
+    end
+  | _ := fail "target is not an equation"
+  end
 
 namespace tactic.interactive
 
-open tidy.rewrite_search
-open interactive interactive.types expr tactic
-
-meta def rewrite_search (rs: parse rw_rules) (cfg : rewrite_search_config := {}) : tactic string :=
-do rs ← rs.rules.mmap (λ r, do e ← to_expr' r.rule, pure (e, r.symm)),
-   rewrite_search_target rs cfg
-
--- meta def mk_app_aux : expr → expr → expr → tactic expr
---  | f (expr.pi n binder_info.default d b) arg := do
---    infer_type arg >>= unify d,
---    return $ f arg
---  | f (expr.pi n _ d b) arg := do
---    v ← mk_meta_var d,
---    t ← whnf (b.instantiate_var v),
---    mk_app_aux (f v) t arg
---  | e _ _ := failed
-
--- meta def mk_app' (f arg : expr) : tactic expr :=
--- do --trace f, trace arg,
---    t ← infer_type f >>= whnf,
---    mk_app_aux f t arg
-
--- meta def apps (e : expr) (F : list expr) : tactic (list expr) :=
--- -- lock_tactic_state $
--- do l ← F.mmap $ λ f, (do r ← try_core (mk_app' e f), return r.to_list), return l.join
-
--- meta def pairwise_apps (E F : list expr) : tactic (list expr) :=
--- (E.mmap $ λ e, apps e F) >>= λ l, return l.join
-
--- meta def close_under_apps_aux : list expr → list expr → tactic (list expr) 
--- | old []  := return old
--- | old new := do oldnew ← pairwise_apps old new,
---                 newold ← pairwise_apps new old,
---                 newnew ← pairwise_apps new new,
---                 close_under_apps_aux (old ++ new) (oldnew ++ newold ++ newnew)
-
--- meta def close_under_apps (E : list expr) : tactic (list expr) := close_under_apps_aux [] E
+meta def rewrite_search (rs: parse rw_rules) (cfg : config := {}) : tactic string := do
+  rs ← rs.rules.mmap (λ r, do e ← to_expr' r.rule, pure (e, r.symm)),
+  do_rewrite_search rs cfg
 
 meta def is_eq_after_binders : expr → bool
-| (expr.pi n bi d b) := is_eq_after_binders b
-| `(%%a = %%b)       := tt
-| _                  := ff
+  | (expr.pi n bi d b) := is_eq_after_binders b
+  | `(%%a = %%b)       := tt
+  | _                  := ff
 
-meta def rewrite_search_using (a : name) (cfg : rewrite_search_config := {}) : tactic string :=
+meta def rewrite_search_using (a : name) (cfg : config := {}) : tactic string :=
 do names ← attribute.get_instances a,
-   exprs ← names.mmap $ mk_const,
-   hyps ← local_context,
-   let exprs := exprs ++ hyps,
+  exprs ← names.mmap $ mk_const,
+  hyps ← local_context,
+  let exprs := exprs ++ hyps,
   --  rules ← close_under_apps exprs, -- TODO don't do this for everything, it's too expensive: only for specially marked lemmas
-   let rules := exprs,
-   rules ← rules.mfilter $ λ r, (do t ← infer_type r, return (is_eq_after_binders t)),
-   let pairs := rules.map (λ e, (e, ff)) ++ rules.map (λ e, (e, tt)),
-   rewrite_search_target pairs cfg
+  let rules := exprs,
+  rules ← rules.mfilter $ λ r, (do t ← infer_type r, return (is_eq_after_binders t)),
+  let pairs := rules.map (λ e, (e, ff)) ++ rules.map (λ e, (e, tt)),
+  do_rewrite_search pairs cfg
 
 end tactic.interactive
 
@@ -277,22 +70,3 @@ meta def search_attribute : user_attribute := {
 }
 
 run_cmd attribute.register `search_attribute
-
--- structure cat :=
---   (O : Type)
---   (H : O → O → Type)
---   (i : Π o : O, H o o)
---   (c : Π {X Y Z : O} (f : H X Y) (g : H Y Z), H X Z)
---   (li : Π {X Y : O} (f : H X Y), c (i X) f = f)
---   (ri : Π {X Y : O} (f : H X Y), c f (i Y) = f)
---   (a : Π {W X Y Z : O} (f : H W X) (g : H X Y) (h : H Y Z), c (c f g) h = c f (c g h))
-
--- attribute [search] cat.li cat.a
-
--- private example (C : cat) (X Y Z : C.O) (f : C.H X Y) (g : C.H Y X) (w : C.c g f = C.i Y) (h k : C.H Y Z) (p : C.c f h = C.c f k) : h = k := 
--- begin
--- rewrite_search_using `search {trace := tt, trace_rules:=tt},
--- end
-
-
--- PROJECT cache all_rewrites_list?
