src/tidy/lib.lean
@@ -1,0 +1,25 @@
+--FIXME the fact that we use this is really sad (ARRAYS DO IT)
+def list_at {α : Type} (default : α) : list α → ℕ → α
+| [] _ := default -- FIXME catastrophic failure
+| (a :: rest) k := if k = 0 then a else list_at rest (k - 1)
+
+def list_set_at_aux {α : Type} (val : α) : list α → list α → ℕ → list α
+| _ [] _          := [] -- FIXME catastrophic failure
+| l (a :: rest) 0 := l.append (val :: rest)
+| l (a :: rest) k := list_set_at_aux (l.append [a]) rest (k - 1)
+
+--FIXME the fact that we use this is really sad (ARRAYS DO IT)
+def list_set_at {α : Type} (l : list α) (idx : ℕ) (val : α) : list α :=
+  list_set_at_aux val [] l idx
+
+def list.split_on_aux {α} [decidable_eq α] (a : α) : list α → list α → list (list α) 
+| [] l       := [l.reverse]
+| (h :: t) l := if h = a then
+                  l.reverse :: (list.split_on_aux t [])
+                else
+                  list.split_on_aux t (h :: l)
+
+def list.split_on {α} [decidable_eq α] (a : α) : list α → list (list α) 
+| l := list.split_on_aux a l []
+
+def string.split_on (c : char) (s : string) := (s.to_list.split_on c).map(λ l, l.as_string)
