src/tidy/rewrite_search/engine.lean
@@ -1,0 +1,482 @@
+import data.list
+import data.option
+
+import tidy.lib
+import .pretty_print
+import .rewrite_all
+
+namespace tidy.rewrite_search
+
+inductive side
+  | L
+  | R
+def side.other : side → side
+  | side.L := side.R
+  | side.R := side.L
+def side.to_string : side → string
+  | side.L := "L"
+  | side.R := "R"
+
+inductive search_result
+  | success : string → search_result
+  | failure : string → search_result
+
+-- universe variables u v
+-- Workaround for the crazy fact that you are only allowed a single universe
+-- in a "do" block. (NOOOOOooooooooo......... (it's getting quieter because
+-- I'm moving on with life.))
+-- meta def pl {α : Type u} (a : α) : tactic (ulift α) := pure (ulift.up a)
+-- meta def ul {α : Type u} {β : Type v} (a : tactic α) : tactic (ulift α) := ulift.up a
+
+-- meta def bound_numeric := ℕ
+inductive bound_progress {β : Type}
+  | exactly : ℕ → bound_progress
+  | at_least : ℕ → β → bound_progress
+open bound_progress
+def bound_progress.bound {β : Type} : @bound_progress β → ℕ
+  | (exactly n)    := n
+  | (at_least n _) := n
+def bound_progress.sure {β : Type} : @bound_progress β → bool
+  | (exactly _)    := tt
+  | (at_least _ _) := ff
+def bound_progress.to_string {β : Type} : @bound_progress β → string
+  | (exactly n)    := "=" ++ to_string n
+  | (at_least n _) := "≥" ++ to_string n
+
+meta def tokenise_expr (e : expr) : tactic (string × list string) := do
+  pp ← pretty_print e,
+  pure (pp, pp.split_on ' ')
+
+def vertex_ref : Type := ℕ
+def vertex_ref_from_nat (r : ℕ) : vertex_ref := r
+def vertex_ref.to_nat (r : vertex_ref) : ℕ := r
+def vertex_ref.to_string (r : vertex_ref) : string := to_string r.to_nat
+def vertex_ref.next (r : vertex_ref) : vertex_ref := vertex_ref_from_nat (r + 1)
+def mk_vertex_ref_null : vertex_ref := vertex_ref_from_nat 0x8FFFFFFF
+def mk_vertex_ref_first : vertex_ref := vertex_ref_from_nat 0
+
+meta structure edge :=
+  (f t   : vertex_ref)
+  (proof : expr)
+  (how   : ℕ)
+
+meta structure vertex :=
+  (id      : vertex_ref)
+  (exp     : expr)
+  (pp      : string)
+  (tokens  : list string)
+
+  (root    : bool)
+  (visited : bool)
+  (s       : option side)
+  (parent  : option edge)
+  (adj     : list edge)
+
+--FIXME do this better with decidability
+meta def vertex.same_side (a b : vertex) : bool :=
+  match (a.s, b.s) with
+    | (some side.L, some side.L) := tt
+    | (some side.R, some side.R) := tt
+    | _ := ff
+  end
+
+meta def vertex.to_string (v : vertex) : string :=
+  let pfx : string := match v.s with
+    | (some s) := s.to_string
+    | none := "?"
+  end in
+  pfx ++ v.pp
+
+meta def null_expr : expr := default expr
+meta def mk_null_vertex : vertex :=
+  ⟨ mk_vertex_ref_null, null_expr, "__NULLEXPR", [], ff, ff, side.L, none, [] ⟩
+
+structure dist_estimate (state_type : Type) :=
+  (l r : vertex_ref)
+  (bnd : @bound_progress state_type)
+def dist_estimate.side {α : Type} (de : dist_estimate α) (s : side) : vertex_ref :=
+  match s with
+  | side.L := de.l
+  | side.R := de.r
+  end
+def dist_estimate.to_string {α : Type} (de : dist_estimate α) : string :=
+  (de.l.to_string) ++ "-" ++ (de.r.to_string) ++ "Δ" ++ de.bnd.to_string
+
+meta def init_bound_fn (β : Type) := vertex → vertex → @bound_progress β
+meta def improve_estimate_fn (β : Type) := ℕ → vertex → vertex → @bound_progress β → @bound_progress β
+
+meta inductive status
+  | going : ℕ → status
+  | done : edge → status
+  | abort
+meta def status.next_itr : status → status
+  | (status.going n) := status.going (n + 1)
+  | other := other
+
+meta structure global_state (α β : Type) :=
+  (next_id  : vertex_ref)
+  (vertices : list vertex) -- FIXME use array
+
+  (estimates : list (dist_estimate β))
+  (interesting_pairs : list (dist_estimate β))
+
+  (solving_edge : option edge)
+  (internal_strat_state : α)
+
+-- Retrieve the vertex with the given ref, or the null vertex if it is not
+-- present.
+meta def global_state.get_vertex {α β : Type} (g : global_state α β) (r : vertex_ref) : vertex :=
+  list_at mk_null_vertex g.vertices r
+
+meta def global_state.set_vertex {α β : Type} (g : global_state α β) (v : vertex) : (global_state α β) :=
+  ⟨ g.next_id, list_set_at g.vertices v.id v, g.estimates, g.interesting_pairs, g.solving_edge, g.internal_strat_state ⟩
+
+meta def global_state.get_endpoints {α β : Type} (g : global_state α β) (e : edge) : vertex × vertex :=
+  (g.get_vertex e.f, g.get_vertex e.t)
+
+meta def global_state.get_estimate_verts {α β : Type} (g : global_state α β) (de : dist_estimate β) : vertex × vertex :=
+  (g.get_vertex de.l, g.get_vertex de.r)
+
+meta def dump_rws : list (expr × expr × ℕ × ℕ) → tactic unit
+  | [] := tactic.trace ""
+  | (a :: rest) := do tactic.trace format!"→{a.1}\nPF:{a.2}", dump_rws rest
+
+meta def dump_vertices : list vertex → tactic unit
+  | [] := tactic.trace ""
+  | (a :: rest) := do
+    let pfx : string := match a.parent with
+      | none := "?"
+      | some p := p.f.to_string
+    end,
+    tactic.trace format!"V{a.id.to_string}:{a.pp}<-{pfx}",
+    dump_vertices rest
+
+meta def dump_estimates {α β : Type} (g : global_state α β) : list (dist_estimate β) → tactic unit
+  | [] := tactic.trace ""
+  | (a :: rest) := do
+  tactic.trace format!"I{(g.get_vertex a.l).pp}-{(g.get_vertex a.r).pp}:{a.bnd.bound}",
+  dump_estimates rest
+  
+-- Forcibly add a new vertex to the vertex table. Probably should never be 
+-- called by a strategy and add_vertex to should used instead.
+meta def global_state.do_alloc_vertex {α β : Type} (g : global_state α β) (e : expr) (root : bool) (s : option side)
+  : tactic (global_state α β × vertex) := do
+  (pp, tokens) ← tokenise_expr e,
+  let v : vertex := ⟨ g.next_id, e, pp, tokens, root, ff, s, none, [] ⟩,
+  return (⟨ g.next_id.next, g.vertices.append [v], g.estimates, g.interesting_pairs, g.solving_edge,g.internal_strat_state ⟩, v)
+  
+-- Forcibly add a new pair to the interesting pair list. Probably should never be 
+-- called by a strategy and add_vertex to should used instead.
+meta def global_state.do_alloc_pair {α β : Type} (g : global_state α β) (de : dist_estimate β)
+  : tactic (global_state α β) := do
+  return (⟨ g.next_id, g.vertices, g.estimates.append [de], g.interesting_pairs.append [de], g.solving_edge, g.internal_strat_state ⟩)
+
+meta def global_state_find_vertex_aux (pp : string) : list vertex → option vertex
+| [] := none
+| (a :: rest) := if a.pp = pp then some a else global_state_find_vertex_aux rest
+
+-- Find the vertex with the given (e : expr), or return the null verterx if not
+-- found.
+meta def global_state.find_vertex {α β : Type} (g : global_state α β) (e : expr) : tactic (option vertex) := do
+  pp ← pretty_print e,
+  return (global_state_find_vertex_aux pp g.vertices)
+
+meta def global_state_find_pair_aux {β : Type} (l r : vertex_ref) : list (dist_estimate β) → option (dist_estimate β)
+| [] := none
+| (a :: rest) :=
+  if (a.l = l ∧ a.r = r) ∨ (a.l = r ∧ a.r = l) then
+    some a
+  else
+    global_state_find_pair_aux rest
+
+-- Find the vertex with the given (e : expr), or return the null verterx if not
+-- found.
+meta def global_state.find_pair {α β : Type} (g : global_state α β) (l r : vertex_ref) : option (dist_estimate β) :=
+  global_state_find_pair_aux l r g.estimates
+
+meta def global_state.register_solved {α β : Type} (g : global_state α β) (e : edge) : global_state α β :=
+  ⟨ g.next_id, g.vertices, g.estimates, g.interesting_pairs, some e, g.internal_strat_state ⟩
+
+-- Look up the given vertex associated to (e : expr), or create it if it is
+-- not already present.
+meta def global_state.do_add_vertex {α β : Type} (g : global_state α β) (e : expr) (root : bool) (s : option side)
+  : tactic (global_state α β × vertex) := do
+  maybe_v ← g.find_vertex e,
+  match maybe_v with
+    | none := do
+      (g, v) ← g.do_alloc_vertex e root s,
+      -- tactic.trace format!"addV: {v.pp}",
+      return (g, v)
+    | (some v) := return (g, v)
+  end
+
+meta def global_state.add_vertex {α β : Type} (g : global_state α β) (e : expr) :=
+  global_state.do_add_vertex g e ff none
+
+meta def global_state.add_root_vertex {α β : Type} (g : global_state α β) (e : expr) (s : side) :=
+  global_state.do_add_vertex g e tt s
+
+meta def global_state.add_adj {α β : Type} (g : global_state α β) (v : vertex)
+  (e : edge) : tactic (global_state α β × vertex) := do
+  let v : vertex := ⟨ v.id, v.exp, v.pp, v.tokens, v.visited, v.root, v.s, v.parent, v.adj.append [e] ⟩,
+  return (g.set_vertex v, v)
+
+meta def global_state.publish_parent {α β : Type} (f t : vertex) (g : global_state α β)
+  (e : edge) : tactic (global_state α β × vertex) :=
+  if t.root then
+    return (g, t)
+  else
+  match t.parent with
+    | some parent := return (g, t)
+    | none := do
+      let t : vertex := ⟨ t.id, t.exp, t.pp, t.tokens, t.root, t.visited, f.s, some e, t.adj ⟩,
+      return (g.set_vertex t, t)
+  end
+
+meta def global_state.mark_vertex_visited {α β : Type} (g : global_state α β) (vr : vertex_ref)
+  : global_state α β :=
+  let v := g.get_vertex vr in
+  g.set_vertex ⟨ v.id, v.exp, v.pp, v.tokens, v.root, tt, v.s, v.parent, v.adj ⟩
+
+meta def global_state.add_edge {α β : Type} (g : global_state α β) (f t : vertex)
+  (proof : expr) (how : ℕ) : tactic (global_state α β × edge) := do
+  let new_edge : edge := ⟨ f.id, t.id, proof, how ⟩,
+  -- tactic.trace format!"addE:{f.to_string}→{t.to_string}",
+  (g, f) ← g.add_adj f new_edge,
+  (g, t) ← g.add_adj t new_edge,
+  (g, t) ← g.publish_parent f t new_edge,
+  if ¬(vertex.same_side f t) then
+    return (g.register_solved new_edge, new_edge)
+  else
+    return (g, new_edge)
+
+-- updates rival's estimate trying to beat candidate's estimate, stopping if we do or we can't
+-- go any further. We return true if we were able to beat candidate.
+meta def try_to_beat {β : Type} (fn : @improve_estimate_fn β) (candidate rival : @bound_progress β)
+  (rival_l rival_r : vertex) : @bound_progress β × bool :=
+  let m := candidate.bound in
+  match rival with
+  | exactly n := (rival, n <= m)
+  | at_least n p :=
+    let attempt := fn m rival_l rival_r rival in
+    (attempt, attempt.bound < m)
+  end
+
+-- First is closer
+meta def sort_most_interesting {α β : Type} (g : global_state α β) (fn : @improve_estimate_fn β)
+  : dist_estimate β → dist_estimate β → tactic (dist_estimate β × dist_estimate β)
+  | a b := do
+  match try_to_beat fn a.bnd b.bnd (g.get_vertex b.l) (g.get_vertex b.r) with
+    -- b is guarenteed closer, so return it:
+    | (new_b, ff) := return (⟨ b.l, b.r, new_b ⟩, a)
+    -- otherwise:
+    | (new_b, tt) := match a.bnd with
+      -- b is further than the current estimate for a and the estimate for a is exact:
+      | exactly k    := return (a, ⟨ b.l, b.r, new_b ⟩)
+      -- or, b is futher than the current estimate for a but a might actually be worse, so check:
+      | at_least k p := sort_most_interesting ⟨ b.l, b.r, new_b ⟩ a
+    end
+  end
+
+meta def find_most_interesting_aux {α β : Type} (g : global_state α β) (fn : @improve_estimate_fn β)
+  : dist_estimate β → list (dist_estimate β) → list (dist_estimate β) → tactic (dist_estimate β × list (dist_estimate β))
+  | current_best seen [] := return (current_best, seen)
+  | current_best seen (a :: rest) := do
+    (vl, vr) ← pure (g.get_estimate_verts a),
+    -- Drop "interesting" vertices which have had both ends visited, and hence aren't interesting
+    -- any more.
+    if vl.visited ∧ vr.visited then
+      find_most_interesting_aux current_best seen rest
+    else do
+      (better, worse) ← sort_most_interesting g fn current_best a,
+      r ← find_most_interesting_aux better (worse :: seen) rest,
+      return r
+
+meta def find_most_interesting {α β : Type} (g : global_state α β) (fn : @improve_estimate_fn β)
+  : list (dist_estimate β) → tactic (list (dist_estimate β))
+  | [] := return []
+  | (a :: rest) := do
+    (vl, vr) ← pure (g.get_estimate_verts a),
+    if vl.visited ∧ vr.visited then
+      find_most_interesting rest
+    else do
+      (best, others) ← find_most_interesting_aux g fn a [] rest,
+      return (best :: others)
+
+meta def global_state.find_most_interesting {α β : Type} (g : global_state α β) (fn : @improve_estimate_fn β) : tactic (global_state α β) := do
+  -- dump_estimates g g.interesting_pairs,
+  new_interestings ← find_most_interesting g fn g.interesting_pairs,
+  return ⟨ g.next_id, g.vertices, g.estimates, new_interestings, g.solving_edge, g.internal_strat_state ⟩ 
+
+meta def refresh_fn (α β : Type) : Type :=
+  global_state α β → global_state α β
+
+meta inductive strategy_action {α β : Type}
+  | examine : dist_estimate β → side → strategy_action
+  | refresh : refresh_fn α β → strategy_action
+  | abort   : string → strategy_action
+open strategy_action
+
+meta def step_fn (α β : Type) : Type := global_state α β → ℕ → global_state α β × (@strategy_action α β)
+
+meta structure strategy {α β : Type} :=
+  (init : α)
+  (step : step_fn α β)
+
+  (init_bound : init_bound_fn β)
+  (improve_estimate_over : improve_estimate_fn β)
+
+structure config := 
+  (trace : bool := ff)
+
+meta structure inst (α β : Type) :=
+  (conf  : config)
+  (rs    : list (expr × bool))
+  (strat : @strategy α β)
+  (g     : global_state α β)
+
+meta def inst.mutate {α β : Type} (i : inst α β) (g : global_state α β) : inst α β :=
+  ⟨ i.conf, i.rs, i.strat, g ⟩
+
+-- Add an "interesting pair" to the global state
+meta def inst.add_pair {α β : Type} (i : inst α β) (l r : vertex) : tactic (inst α β) := do
+  -- tactic.trace format!"add_pair:({l.pp}, {r.pp})",
+  match i.g.find_pair l.id r.id with
+    | some de := return i
+    | none := do
+        g ← i.g.do_alloc_pair ⟨ l.id, r.id, i.strat.init_bound l r ⟩,
+        return (i.mutate g)
+    end
+
+meta def inst.find_most_interesting {α β : Type} (i : inst α β) : tactic (inst α β) := do
+  g ← i.g.find_most_interesting i.strat.improve_estimate_over,
+  return (i.mutate g)
+
+meta def store_new_equalities {α β : Type} (f : vertex) : global_state α β → list (expr × expr × ℕ × ℕ) → tactic (global_state α β × list vertex × list edge)
+  | g [] := return (g, [], [])
+  | g ((new_expr, prf, i, j) :: rest) := do
+      (g, v) ← g.add_vertex new_expr,
+      (g, e) ← g.add_edge f v prf i,
+      (g, vs, es) ← store_new_equalities g rest,
+      return (g, (v :: vs), (e :: es))
+
+meta def add_new_interestings {α β : Type} (v : vertex) : inst α β → list vertex → tactic (inst α β)
+  | i [] := return i
+  | i (a :: rest) := do
+      i ← i.add_pair v a,
+      add_new_interestings i rest
+
+-- My job is to examine the specified side and to blow up the vertex once
+meta def inst.examine_one {α β : Type} (i : inst α β) (de : dist_estimate β) (s : side) : tactic (inst α β) := do
+  let v := i.g.get_vertex (de.side s),
+  all_rws ← all_rewrites_list i.rs v.exp,
+  (g, touched_verts, new_edges) ← store_new_equalities v i.g all_rws,
+  g ← pure (g.mark_vertex_visited v.id),
+  i ← pure (i.mutate g),
+  i ← add_new_interestings (i.g.get_vertex (de.side s.other)) i touched_verts,
+  i ← i.find_most_interesting,
+  return i
+
+meta def inst.step_once {α β : Type} (i : inst α β) (itr : ℕ) : tactic (inst α β × status) :=
+  match i.g.solving_edge with
+  | some e := return (i, status.done e)
+  | none :=
+    let (g, action) := i.strat.step i.g itr in
+    let i := i.mutate g in
+    match action with
+      | examine de s := do
+        target ← pure (g.get_vertex (de.side s)),
+        buddy ← pure (g.get_vertex (de.side s.other)),
+        tactic.trace format!"examine {target.pp}-{buddy.pp}",
+        -- dump_vertices g.vertices,
+        -- dump_estimates g g.interesting_pairs,
+        if target.visited then do
+          tactic.trace format!"abort: already visited vertex!",
+          return (i, status.abort)
+        else do
+          i ← i.examine_one de s,
+          return (i, status.going (itr + 1))
+      | refresh ref_fn := do
+        tactic.trace format!"refresh",
+        return (i.mutate (ref_fn i.g), status.going (itr + 1))
+      | abort reason := do
+        tactic.trace format!"abort: {reason}",
+        return (i, status.abort)
+    end
+  end
+
+meta def inst.backtrack_to_root_with {α β : Type} (i : inst α β) : vertex → expr → tactic expr :=
+  λ (cur : vertex) (prf_so_far : expr), do
+  match cur.parent with
+    | none := return prf_so_far
+    | some e := do
+      let parent : vertex := i.g.get_vertex e.f,
+      new_expr ← tactic.mk_eq_trans e.proof prf_so_far,
+      inst.backtrack_to_root_with parent new_expr
+  end
+
+--FIXME code duplication with above
+meta def inst.backtrack_to_root {α β : Type} (i : inst α β) (cur : vertex) : tactic (option expr) := do
+  match cur.parent with
+    | none := return none
+    | some e := do
+      let parent : vertex := i.g.get_vertex e.f,
+      proof ← i.backtrack_to_root_with parent e.proof,
+      return proof
+  end
+
+meta def flip_half (h : expr) : tactic expr := tactic.mk_eq_symm h
+meta def unify_halves (l r : expr) : tactic expr := tactic.mk_eq_trans l r
+
+meta def inst.solve_goal {α β : Type} (i : inst α β) (e : edge) : tactic string := do
+  let (vf, vt) := i.g.get_endpoints e,
+  
+  rhs_half ← i.backtrack_to_root_with vf e.proof,
+  rhs_half ← flip_half rhs_half,
+
+  lhs_half ← i.backtrack_to_root vt,
+  match lhs_half with
+    | some lhs_half := do
+      proof ← unify_halves lhs_half rhs_half,
+      proof ← match vf.s with
+        | some side.L := tactic.mk_eq_symm proof
+        | _           := pure proof
+      end,
+
+      pp ← pretty_print proof,
+      tactic.trace pp,
+      tactic.trace vf.to_string,
+      tactic.trace vt.to_string,
+
+      tactic.exact proof
+    | none := tactic.skip
+  end,
+
+  return "aaaaaa pretty version"
+
+meta def inst.search_until_stop_aux {α β : Type} : inst α β → ℕ → tactic search_result := λ i itr, do
+  (i, s) ← i.step_once itr,
+  match s with
+    | status.going k := inst.search_until_stop_aux i (itr + 1)
+    | status.abort   := return (search_result.failure "aborted")
+    | status.done e  := do
+      str ← i.solve_goal e,
+      return (search_result.success str)
+  end
+
+meta def inst.search_until_abort {α β : Type} (i : inst α β) : tactic search_result :=
+  i.search_until_stop_aux 0
+
+meta def mk_initial_global_state {α β : Type} (strat : @strategy α β) : global_state α β :=
+  ⟨ mk_vertex_ref_first, [], [], [], none, strat.init ⟩
+
+meta def mk_search_instance {α β : Type} (conf : config) (rs : list (expr × bool)) (strat : @strategy α β) (lhs rhs : expr)
+  : tactic (inst α β) := do
+  let g := mk_initial_global_state strat,
+  (g, vl) ← g.add_root_vertex lhs side.L,
+  (g, vr) ← g.add_root_vertex rhs side.R,
+  let i := inst.mk conf rs strat g,
+  i ← i.add_pair vl vr,
+  return i
+
+end tidy.rewrite_search
