src/tidy/rewrite_search/strategy/edit_distance.lean
@@ -1,0 +1,77 @@
+import tidy.rewrite_search.engine
+
+open tidy.rewrite_search
+open tidy.rewrite_search.bound_progress
+
+namespace tidy.rewrite_search.strategy.edit_distance
+
+variables {α : Type} [decidable_eq α]
+
+meta structure ed_searchstate :=
+  (dummy : ℕ)
+
+@[derive decidable_eq]
+structure ed_partial := 
+  (prefix_length : ℕ)
+  (suffix    : list string)
+  (distances : list ℕ) -- distances from the prefix of l₁ to each non-empty prefix of l₂
+
+def empty_partial_edit_distance_data (l₁ l₂: list string) : ed_partial :=
+  ⟨ 0, l₁, (list.range l₂.length).map(λ n, n + 1) ⟩
+
+meta def ed_searchstate_init : ed_searchstate := ⟨ 1 ⟩
+
+meta def ed_step (g : global_state ed_searchstate ed_partial) (itr : ℕ)
+  : global_state ed_searchstate ed_partial × (@strategy_action ed_searchstate ed_partial) :=
+  if itr <= 10 then
+    match g.interesting_pairs with
+    | [] := (g, strategy_action.abort "all interesting pairs exhausted!")
+    | (best_p :: rest) :=
+      let vl := g.get_vertex (best_p.side side.L) in
+      let s : side := if itr % 2 = 0 ∧ ¬vl.visited then side.L else side.R in
+      (g, strategy_action.examine best_p s)
+    end
+  else
+    (g, strategy_action.abort "max iterations reached")
+
+meta def ed_init_bound (l r : vertex) : @bound_progress ed_partial :=
+  at_least 0 (empty_partial_edit_distance_data l.tokens r.tokens)
+
+def triples {α : Type} (p : ed_partial) (l₂ : list α): list (ℕ × ℕ × α) := p.distances.zip ((p.prefix_length :: p.distances).zip l₂)
+
+--FIXME rewrite me
+meta def fold_fn (h : string) (n : ℕ × list ℕ) (t : ℕ × ℕ × string) := 
+  let m := (if h = t.2.2 then t.2.1 else 1 + min (min (t.2.1) (t.1)) n.2.head) in 
+  (min m n.1, m :: n.2)
+
+--FIXME rewrite me
+meta def ed_improve_bound_once (l r : list string) (cur : ℕ) (p : ed_partial) : @bound_progress ed_partial :=
+  match p.suffix with
+    | [] := exactly p.distances.ilast
+    | (h :: t) :=
+      let initial := (p.prefix_length + 1, [p.prefix_length + 1]) in
+      let new_distances : ℕ × list ℕ := (triples p r).foldl (fold_fn h) initial in
+      at_least new_distances.1 ⟨ p.prefix_length + 1, t, new_distances.2.reverse.drop 1 ⟩
+  end 
+
+meta def ed_improve_bound_over (l r : list string) (m : ℕ) : @bound_progress ed_partial → @bound_progress ed_partial
+| (exactly n) := exactly n
+| (at_least n p) :=
+  if n > m then
+    at_least n p
+  else
+    ed_improve_bound_over (ed_improve_bound_once l r n p)
+
+meta def ed_improve_estimate_over (m : ℕ) (l r : vertex) (bnd : @bound_progress ed_partial) : @bound_progress ed_partial :=
+  ed_improve_bound_over l.tokens r.tokens m bnd
+
+end tidy.rewrite_search.strategy.edit_distance
+
+namespace tidy.rewrite_search.strategy
+
+open tidy.rewrite_search.strategy.edit_distance
+
+meta def edit_distance_strategy : @strategy ed_searchstate ed_partial :=
+  ⟨ ed_searchstate_init, ed_step, ed_init_bound, ed_improve_estimate_over ⟩
+
+end tidy.rewrite_search.strategy
