test/rewrite_search.lean
@@ -115,4 +115,12 @@ constants f g : ℕ → ℕ → ℕ → ℕ
 
 lemma test : f 0 0 0 = g 0 0 0 := by rewrite_search_using `search {trace := tt}
 
+constant h : ℕ → ℕ
+@[search,simp] axiom a1 : h 0 = h 1
+@[search,simp] axiom a2 : h 1 = h 2
+@[search,simp] axiom a3 : h 2 = h 3
+@[search,simp] axiom a4 : h 3 = h 4
+
+lemma test2 : h 0 = h 4 := by rewrite_search_using `search {trace := tt}
+
 end tidy.rewrite_search.examples
